proofs/Axioms.lean
@@ -18,3 +18,4 @@ import Statements
 #print axioms Protocol.Statements.check_C2_decode
 #print axioms Protocol.Statements.check_S1_S2_decode
 #print axioms Protocol.Statements.check_S2_signed_len
+#print axioms Protocol.Statements.check_S13_valid_id
